Ints/num/W.v
@@ -24,25 +24,25 @@ Defined.
 
 (* Make the op *)
 
-Fixpoint mk_op (w : Type) (op : znz_op w) (n : nat) {struct n} :
-  znz_op (word w n) :=
-  match n return (znz_op (word w n)) with
+Fixpoint mk_op (w : Type) (op : ZnZ.Ops w) (n : nat) {struct n} :
+  ZnZ.Ops (word w n) :=
+  match n return (ZnZ.Ops (word w n)) with
   | O => op
-  | S n1 => mk_zn2z_op_karatsuba (mk_op op n1)
+  | S n1 => mk_zn2z_ops_karatsuba (mk_op op n1)
   end.
 
-Theorem mk_op_digits: forall w (op: znz_op w) n, 
-  (Zpos (znz_digits (mk_op op n)) = 2 ^ Z_of_nat n * Zpos (znz_digits op))%Z.
+Theorem mk_op_digits: forall w (op: ZnZ.Ops w) n, 
+  (Zpos (ZnZ.digits (mk_op op n)) = 2 ^ Z_of_nat n * Zpos (ZnZ.digits op))%Z.
 intros w op n; elim n; simpl mk_op; auto; clear n.
-intros n Rec; simpl znz_digits.
+intros n Rec; simpl ZnZ.digits.
 rewrite Zpos_xO; rewrite Rec.
 rewrite Zmult_assoc; apply f_equal2 with (f := Zmult); auto.
 rewrite inj_S; unfold Zsucc; rewrite Zplus_comm.
 rewrite Zpower_exp; auto with zarith.
 Qed.
 
-Theorem digits_pos: forall w (op: znz_op w) n,
-  (1 < Zpos (znz_digits op) ->  1 < Zpos (znz_digits (mk_op op n)))%Z.
+Theorem digits_pos: forall w (op: ZnZ.Ops w) n,
+  (1 < Zpos (ZnZ.digits op) ->  1 < Zpos (ZnZ.digits (mk_op op n)))%Z.
 intros w op n H.
 rewrite mk_op_digits.
 rewrite <- (Zmult_1_r 1).
@@ -53,101 +53,101 @@ apply Zpower_le_monotone; auto with zarith.
 apply Zmult_lt_compat_l; auto with zarith.
 Qed.
 
-Fixpoint mk_spec (w : Type) (op : znz_op w) (op_spec : znz_spec op) 
-    (H: (1 < Zpos (znz_digits op))%Z)  (n : nat)
-            {struct n} : znz_spec (mk_op op n) :=
-  match n return (znz_spec (mk_op op n)) with
+Fixpoint mk_spec (w : Type) (op : ZnZ.Ops w) (op_spec : ZnZ.Specs op) 
+    (H: (1 < Zpos (ZnZ.digits op))%Z)  (n : nat)
+            {struct n} : ZnZ.Specs (mk_op op n) :=
+  match n return (ZnZ.Specs (mk_op op n)) with
   | O => op_spec
   | S n1 =>
-      @mk_znz2_karatsuba_spec (word w n1) (mk_op op n1)
+      @mk_zn2z_specs_karatsuba (word w n1) (mk_op op n1)
         (* (digits_pos op n1 H) *) (mk_spec op_spec H n1)
   end.
 
 (* ** Operators ** *)
-Definition w31_1_op := mk_zn2z_op int31_op.           
-Definition w31_2_op := mk_zn2z_op w31_1_op.
-Definition w31_3_op := mk_zn2z_op w31_2_op.
-Definition w31_4_op := mk_zn2z_op_karatsuba w31_3_op.
-Definition w31_5_op := mk_zn2z_op_karatsuba w31_4_op.
-Definition w31_6_op := mk_zn2z_op_karatsuba w31_5_op.
-Definition w31_7_op := mk_zn2z_op_karatsuba w31_6_op.
-Definition w31_8_op := mk_zn2z_op_karatsuba w31_7_op.
-Definition w31_9_op := mk_zn2z_op_karatsuba w31_8_op.
-Definition w31_10_op := mk_zn2z_op_karatsuba w31_9_op.
-Definition w31_11_op := mk_zn2z_op_karatsuba w31_10_op.
-Definition w31_12_op := mk_zn2z_op_karatsuba w31_11_op.
-Definition w31_13_op := mk_zn2z_op_karatsuba w31_12_op.
-Definition w31_14_op := mk_zn2z_op_karatsuba w31_13_op.
+Definition w31_1_ops := mk_zn2z_ops int31_ops.           
+Definition w31_2_ops := mk_zn2z_ops w31_1_ops.
+Definition w31_3_ops := mk_zn2z_ops w31_2_ops.
+Definition w31_4_ops := mk_zn2z_ops_karatsuba w31_3_ops.
+Definition w31_5_ops := mk_zn2z_ops_karatsuba w31_4_ops.
+Definition w31_6_ops := mk_zn2z_ops_karatsuba w31_5_ops.
+Definition w31_7_ops := mk_zn2z_ops_karatsuba w31_6_ops.
+Definition w31_8_ops := mk_zn2z_ops_karatsuba w31_7_ops.
+Definition w31_9_ops := mk_zn2z_ops_karatsuba w31_8_ops.
+Definition w31_10_ops := mk_zn2z_ops_karatsuba w31_9_ops.
+Definition w31_11_ops := mk_zn2z_ops_karatsuba w31_10_ops.
+Definition w31_12_ops := mk_zn2z_ops_karatsuba w31_11_ops.
+Definition w31_13_ops := mk_zn2z_ops_karatsuba w31_12_ops.
+Definition w31_14_ops := mk_zn2z_ops_karatsuba w31_13_ops.
 
-Definition cmk_op (n: nat): znz_op (word int31 n).
+Definition cmk_ops (n: nat): ZnZ.Ops (word int31 n).
 intros n; case n; clear n.
-exact int31_op.
+exact int31_ops.
 intros n; case n; clear n.
-exact w31_1_op.
+exact w31_1_ops.
 intros n; case n; clear n.
-exact w31_2_op.
+exact w31_2_ops.
 intros n; case n; clear n.
-exact w31_3_op.
+exact w31_3_ops.
 intros n; case n; clear n.
-exact w31_4_op.
+exact w31_4_ops.
 intros n; case n; clear n.
-exact w31_5_op.
+exact w31_5_ops.
 intros n; case n; clear n.
-exact w31_6_op.
+exact w31_6_ops.
 intros n; case n; clear n.
-exact w31_7_op.
+exact w31_7_ops.
 intros n; case n; clear n.
-exact w31_8_op.
+exact w31_8_ops.
 intros n; case n; clear n.
-exact w31_9_op.
+exact w31_9_ops.
 intros n; case n; clear n.
-exact w31_10_op.
+exact w31_10_ops.
 intros n; case n; clear n.
-exact w31_11_op.
+exact w31_11_ops.
 intros n; case n; clear n.
-exact w31_12_op.
+exact w31_12_ops.
 intros n; case n; clear n.
-exact w31_13_op.
+exact w31_13_ops.
 intros n; case n; clear n.
-exact w31_14_op.
+exact w31_14_ops.
 intros n.
 match goal with |- context[S ?X] =>
- exact (mk_op int31_op (S X))
+ exact (mk_op int31_ops (S X))
 end.
 Defined.
 
-Definition cmk_spec n: znz_spec (cmk_op n).
-assert (S1: znz_spec w31_1_op).
-unfold w31_1_op; apply mk_znz2_spec; auto with zarith.
-exact int31_spec.
-assert (S2: znz_spec w31_2_op).
-unfold w31_2_op; apply mk_znz2_spec; auto with zarith.
-assert (S3: znz_spec w31_3_op).
-unfold w31_3_op; apply mk_znz2_spec; auto with zarith.
-assert (S4: znz_spec w31_4_op).
-unfold w31_4_op; apply mk_znz2_karatsuba_spec; auto with zarith.
-assert (S5: znz_spec w31_5_op).
-unfold w31_5_op; apply mk_znz2_karatsuba_spec; auto with zarith.
-assert (S6: znz_spec w31_6_op).
-unfold w31_6_op; apply mk_znz2_karatsuba_spec; auto with zarith.
-assert (S7: znz_spec w31_7_op).
-unfold w31_7_op; apply mk_znz2_karatsuba_spec; auto with zarith.
-assert (S8: znz_spec w31_8_op).
-unfold w31_8_op; apply mk_znz2_karatsuba_spec; auto with zarith.
-assert (S9: znz_spec w31_9_op).
-unfold w31_9_op; apply mk_znz2_karatsuba_spec; auto with zarith.
-assert (S10: znz_spec w31_10_op).
-unfold w31_10_op; apply mk_znz2_karatsuba_spec; auto with zarith.
-assert (S11: znz_spec w31_11_op).
-unfold w31_11_op; apply mk_znz2_karatsuba_spec; auto with zarith.
-assert (S12: znz_spec w31_12_op).
-unfold w31_12_op; apply mk_znz2_karatsuba_spec; auto with zarith.
-assert (S13: znz_spec w31_13_op).
-unfold w31_13_op; apply mk_znz2_karatsuba_spec; auto with zarith.
-assert (S14: znz_spec w31_14_op).
-unfold w31_14_op; apply mk_znz2_karatsuba_spec; auto with zarith.
+Definition cmk_spec n: ZnZ.Specs (cmk_ops n).
+assert (S1: ZnZ.Specs w31_1_ops).
+unfold w31_1_ops; apply mk_zn2z_specs; auto with zarith.
+exact int31_specs.
+assert (S2: ZnZ.Specs w31_2_ops).
+unfold w31_2_ops; apply mk_zn2z_specs; auto with zarith.
+assert (S3: ZnZ.Specs w31_3_ops).
+unfold w31_3_ops; apply mk_zn2z_specs; auto with zarith.
+assert (S4: ZnZ.Specs w31_4_ops).
+unfold w31_4_ops; apply mk_zn2z_specs_karatsuba; auto with zarith.
+assert (S5: ZnZ.Specs w31_5_ops).
+unfold w31_5_ops; apply mk_zn2z_specs_karatsuba; auto with zarith.
+assert (S6: ZnZ.Specs w31_6_ops).
+unfold w31_6_ops; apply mk_zn2z_specs_karatsuba; auto with zarith.
+assert (S7: ZnZ.Specs w31_7_ops).
+unfold w31_7_ops; apply mk_zn2z_specs_karatsuba; auto with zarith.
+assert (S8: ZnZ.Specs w31_8_ops).
+unfold w31_8_ops; apply mk_zn2z_specs_karatsuba; auto with zarith.
+assert (S9: ZnZ.Specs w31_9_ops).
+unfold w31_9_ops; apply mk_zn2z_specs_karatsuba; auto with zarith.
+assert (S10: ZnZ.Specs w31_10_ops).
+unfold w31_10_ops; apply mk_zn2z_specs_karatsuba; auto with zarith.
+assert (S11: ZnZ.Specs w31_11_ops).
+unfold w31_11_ops; apply mk_zn2z_specs_karatsuba; auto with zarith.
+assert (S12: ZnZ.Specs w31_12_ops).
+unfold w31_12_ops; apply mk_zn2z_specs_karatsuba; auto with zarith.
+assert (S13: ZnZ.Specs w31_13_ops).
+unfold w31_13_ops; apply mk_zn2z_specs_karatsuba; auto with zarith.
+assert (S14: ZnZ.Specs w31_14_ops).
+unfold w31_14_ops; apply mk_zn2z_specs_karatsuba; auto with zarith.
 intros n; case n; clear n.
-exact int31_spec.
+exact int31_specs.
 intros n; case n; clear n.
 exact S1.
 intros n; case n; clear n.
@@ -177,9 +177,10 @@ exact S13.
 intros n; case n; clear n.
 exact S14.
 intro n.
-simpl cmk_op.
-repeat match goal with |- znz_spec (mk_zn2z_op_karatsuba ?X) =>
-  generalize (@mk_znz2_karatsuba_spec _ X); intros tmp;
+simpl cmk_ops.
+repeat match goal with |- ZnZ.Specs
+ (mk_zn2z_ops_karatsuba ?X) =>
+  generalize (@mk_zn2z_specs_karatsuba _ X); intros tmp;
   apply tmp; clear tmp; auto with zarith
 end.
 (*
@@ -187,14 +188,14 @@ apply digits_pos.
 *)
 auto with zarith.
 apply mk_spec.
-exact int31_spec.
+exact int31_specs.
 auto with zarith.
 Defined.
 
 
-Theorem cmk_op_digits: forall n, 
-  (Zpos (znz_digits (cmk_op n)) = 2 ^ (Z_of_nat n) * 31)%Z.
+Theorem cmk_ops_digits: forall n, 
+  (Zpos (ZnZ.digits (cmk_ops n)) = 2 ^ (Z_of_nat n) * 31)%Z.
 do 15 (intros n; case n; clear n; [try reflexivity | idtac]).
-intros n; unfold cmk_op; lazy beta.
+intros n; unfold cmk_ops; lazy beta.
 rewrite mk_op_digits; auto.
 Qed.
